This is the method for solving any cubic equation:

Say we have
!['  ax \^3 + bx \^2 + cx + d = 0  '](../dictionary/equation_images/1989.2..png)\
 Then we define a new variable, y, and set
!['  y = x +   (b)/(3 a)  '](../dictionary/equation_images/1989.3..png)\
 So
!['  x = y - (b)/(3 a),  '](../dictionary/equation_images/1989.4..png)\
 and the equation becomes:
!['  ay \^3   + (c - (b\^2)/(3 a) ) y   + (2 b\^3)/(27 a \^2) - (bc)/(3 a)   + d = 0  '](../dictionary/equation_images/1989.5..png)\
 which we can write as:
!['  y\^3 + py + q = 0  '](../dictionary/equation_images/1989.6..png)\
 by dividing by a and defining p and q appropriately.

Next define two new variables u and v, with
!['  uv = (p)/(3),  '](../dictionary/equation_images/1989.7..png)\
 and !['  y = u - v .  '](../dictionary/equation_images/1989.8..png)\
 So then:
!['  u\^3 - v\^3 + q = 0.  '](../dictionary/equation_images/1989.9..png)\
 But
!['  v = (p)/(3 u),  '](../dictionary/equation_images/1989.10..png)\
 so this becomes:
!['  ( u\^3 ) \^2 + qu\^3 - (p \^3)/(27) = 0  '](../dictionary/equation_images/1989.11..png)\
 which is a quadratic equation in
!['  u\^3 .  '](../dictionary/equation_images/1989.12..png)

We can solve this to find
!['  u\^3 ,  '](../dictionary/equation_images/1989.13..png) so we can
find u, and then v, because
!['  v = (p)/(3 u) .  '](../dictionary/equation_images/1989.14..png)\
 Then we can find y, because
!['  y = u - v,  '](../dictionary/equation_images/1989.15..png)\
 and finally we can find x: \\

![' x =     the (3) th root of (
(- q +  the square root of (q\^2 + (4)/(27) p \^3 ) )/ (2)
)  +   the (3) th root of (
(- q -  the square root of (q\^2 + (4)/(27) p \^3 ) )/ (2) )   - (b)/(3 a) '](../dictionary/equation_images/1989.1..png)

\
 with
!['  p = (c)/(a)   - (b\^2)/(3 a \^2 ),   q = (2 b\^3)/(27 a\^3)  - (bc)/(3 a\^2)   + (d)/(a).  '](../dictionary/equation_images/1989.16..png)
