This is the method for solving any quadratic equation:

Say we have
!['  ax\^2 + bx + c = 0.  '](../dictionary/equation_images/1990.1..png)\
 Then divide by a to get:
!['  x\^2 + (bx)/(a)   + (c)/(a) = 0.  '](../dictionary/equation_images/1990.2..png)\
 Then notice that
!['  ( x + (b)/(2 a) )\^2   = x\^2 + (bx)/(a) + (b\^2)/(4 a\^2)  '](../dictionary/equation_images/1990.3..png)\
 so:
!['  ( x + (b)/(2 a) )\^2   - (b\^2)/(4 a\^2) + (c)/(a) = 0,  '](../dictionary/equation_images/1990.4..png)\

!['  ( x + (b)/(2 a) )\^2   = (b\^2)/(4 a\^2)   - (c)/(a).  '](../dictionary/equation_images/1990.5..png)

So,
!['  x = ( - b (+/-)  the square root of  ( b\^2 - 4 ac) )/  (2 a).  '](../dictionary/equation_images/1990.6..png)

For example, suppose we have 3x^2^+2x-1=0.

Then we divide by 3 to get: x^2^+(2/3)x-(1/3)=0.

Then notice that (x+(1/3))^2^=x^2^+(2/3)x+(1/9)

so: (x+(1/3))^2^-(1/9)-(1/3)=0,

(x+(1/3))^2^=(1/9)+(1/3)=4/9.

So,
!['  x+(1/3)= (+/-) 2/3  '](../dictionary/equation_images/1990.7..png)

!['  x = -1/3 (+/-) 2/3  '](../dictionary/equation_images/1990.8..png)

x=-1 or x=1/3.
