To decompose a fraction is to write it as the sum of a set of partial
fractions. The way to do this is first to factorise the denominator, for
instance we decompose
!['  (1)/(6)  '](../dictionary/equation_images/414.4..png) by noting
that 6=2×3, so
!['  (1)/(6) = (1)/(2) ×  (1)/(3) .  '](../dictionary/equation_images/414.5..png)
This means that we can write
!['  (1)/(6) = A (1)/(2)  + B (1)/(3) .  '](../dictionary/equation_images/414.6..png)

We can find the values of A and B: \\

![' (1)/(6) = A (1)/(2) + B (1)/(3)   = ( 3 A + 2 B )/ (6) '](../dictionary/equation_images/414.1..png)

\\

![' (1)/(6) = ( 3 A + 2 B )/ (6) '](../dictionary/equation_images/414.2..png)

\\

![' 1 = 3 A + 2 B '](../dictionary/equation_images/414.3..png)

- so one solution is A=1, B=-1.

So,
!['  (1)/(6) = (1)/(2) - (1)/(3) .  '](../dictionary/equation_images/414.7..png)

This method can also work when the fraction has polynomials as numerator
and denominator.
