If we write the elliptic integral of the first kind in this form: \\

![' u =  the integral of  \_(0) \^(x) (dt)/   (  the square root of (
((1- t\^2 ) ( 1 - k\^2 t\^2 )
) ) ) , '](../dictionary/equation_images/4472.1..png)

then the elliptic functions sn, cn and dn can be defined as: \\

![' x = sn(u) , '](../dictionary/equation_images/4472.2..png)

\\

!['  the square root of ( 1 - x \^2 ) = cn(u) , '](../dictionary/equation_images/4472.3..png)

\\

!['  the square root of ( 1 - k\^2 x\^2 ) = dn(u) . '](../dictionary/equation_images/4472.4..png)

(This is analogous to defining the circular functions in terms of the
integral
!['  u =  the integral of  \_(0) \^(x) (dt)/  ( the square root of (1-t\^2)
) ,  '](../dictionary/equation_images/4472.5..png) x=sin(u). )
