If we differentiate an implicit equation without first making it
explicit, this is called an implicit differentiation. Very often we have
to use the product rule in order to do this.

For example: !['  xy = 2  '](../dictionary/equation_images/2728.3..png)

Differentiate with respect to x, using the product rule:
!['  (d)/(dx) (xy) = 0  '](../dictionary/equation_images/2728.4..png) \\

![' (dx)/(dx) y + x (dy)/(dx) = 0 '](../dictionary/equation_images/2728.1..png)

\\

![' y + x (dy)/(dx) = 0 '](../dictionary/equation_images/2728.2..png)
