Also called integration by change of variable, integration on
substitution relies on the identity \\

!['  the integral of  f\^( //prime ) (g(x)
) g \^( //prime ) (x) dx = f(g(x)
) + c . '](../dictionary/equation_images/2734.1..png)

Sometimes difficult integrals can be made easier by a carefully-chosen
substitution. For instance: \\

![' I =  the integral of \_0\^1 (1)/( the square root of (1- x\^2)
) dx '](../dictionary/equation_images/2734.2..png)

Let x = sin u, so that \\

![' (dx)/(du) = cos   (u) '](../dictionary/equation_images/2734.3..png)

\
 Then, \\

![' x\^2 +  (  (dx)/(du)  ) \^2  = sin\^2 u + cos\^2 u = 1 '](../dictionary/equation_images/2734.4..png)

\
 So, \\

![' 1- x\^2 = 1 - sin\^2 u = cos\^2 u '](../dictionary/equation_images/2734.5..png)

\
 So, \\

![' I =  the integral of \_(x=0)\^(x=1) (1)/( the square root of (cos\^2 u)
) (cos   (u) ) du '](../dictionary/equation_images/2734.6..png)

\
 \\

![' =  the integral of \_(x=0)\^(x=1) du '](../dictionary/equation_images/2734.7..png)

\
 And when x=0, u=0; when x=1, u=
!['  //pi  '](../dictionary/equation_images/2734.10..png)\
 So, \\

![' I =  the integral of  \_(u=0)\^(u= //pi) du '](../dictionary/equation_images/2734.8..png)

\
 \\

![' = //pi '](../dictionary/equation_images/2734.9..png)
