\\
![' //log \_a ( xy) = //log \_a x + //log \_a y '](../dictionary/equation_images/1616.1..png)
\\
![' //log \_a (x\^n) = n //log \_a x '](../dictionary/equation_images/1616.2..png)
\\
![' //log \_a  ( (1)/(x)  )   = - //log \_a x '](../dictionary/equation_images/1616.3..png)
\\
![' //log \_a a = 1'](../dictionary/equation_images/1616.4..png)
\\
![' //log \_a  ( (x)/(y)  )   = //log \_a x - //log \_a y '](../dictionary/equation_images/1616.5..png)
\\
![' //log \_a  (  the  (n) th root of (x)  )   = (1)/(n) //log \_a x '](../dictionary/equation_images/1616.6..png)
\\
![' //log \_a 1 = 0 '](../dictionary/equation_images/1616.7..png)
\\
![' e\^(ln x ) = x '](../dictionary/equation_images/1616.8..png)
\\
![' ln (e\^x) = x '](../dictionary/equation_images/1616.9..png)
\\
![' //log \_a x = (//log \_b x )/ (//log \_b a ) '](../dictionary/equation_images/1616.10..png)
\\
![' e\^(x ln a ) = a\^x '](../dictionary/equation_images/1616.11..png)
