If X\~B(n,p), ie X is distributed binomially with parameters n and p,
then: \\
![' \< X \> =    the sum of  \_(r=0) \^(n) rp\_(r)  =  the sum of  \_(r=0) \^(n) r   ( //C(n)(r)  ) p \^ (r)  (1- p ) \^ ( n-r) '](../dictionary/equation_images/3425.1..png)
\\
![' =  the sum of  \_(r=1) \^(n) (n!)/(
(r-1)!(n-r)!)  p\^(r) (1-p)\^(n-r) '](../dictionary/equation_images/3425.2..png)
\\
![' = np  the sum of  \_(r=1) \^ (n)  ( (n-1)!)/(
(r-1!)(n-r)!)  p\^(r-1) (1-p) \^ (n-r) '](../dictionary/equation_images/3425.3..png)
\\
![' = np  the sum of  \_(r=0) \^ ( n-1)    ( //C (n-1)(r)  ) p\^(r)  (1-p)\^ (n-1-r) '](../dictionary/equation_images/3425.4..png)
\\
![' = np(p+(1-p) )\^(n-1) '](../dictionary/equation_images/3425.5..png)
\\
![' = np '](../dictionary/equation_images/3425.6..png)
