We know that
!['  \< X \> = np  '](../dictionary/equation_images/3426.9..png) if X is
a random variable binomially distributed with parameters n and p. And:
\\

![' \< X \^2 \> =   the sum of \_(r=0) \^(n) r\^2 p\_(r) '](../dictionary/equation_images/3426.1..png)

\\

![' =  the sum of  \_ (r=0) \^ (n)  r(r-1)  ( //C(n)(r)  )   p\^(r) (1-p) \^(n-r)  +  the sum of  \_ (r=0) \^(n)  r  ( //C(n)(r)  )   p \^(r) (1-p)  \^(n-r) '](../dictionary/equation_images/3426.2..png)

\\

![' = n(n-1)p \^2 + np '](../dictionary/equation_images/3426.3..png)

So, \\

![' var(X) = \< X \^2 \>   - \> X \> \^2 '](../dictionary/equation_images/3426.4..png)

\\

![' = n(n-1)p \^2 + np - n\^2 p\^2 '](../dictionary/equation_images/3426.5..png)

\\

![' = n\^2 p\^2 - np\^2 + np - n\^2 p\^2  '](../dictionary/equation_images/3426.6..png)

\\

![' = np - np\^2 '](../dictionary/equation_images/3426.7..png)

\\

![' = np(1-p) '](../dictionary/equation_images/3426.8..png)
